coq/Addr.v
@@ -1,9 +1,15 @@
-Module Type VADDR.
-  Parameter t:Set.
+Require Import Coq.Numbers.BinNums.
+
+  Module Type VADDR.
+  Parameter Inline t:Set.
 
   Parameter bitwise_complement: t -> t.
 
   Parameter ltb: t -> t -> bool.
   Parameter leb: t -> t -> bool.
   Parameter ltb_irref: forall a:t, ltb a a = false.
+
+  Parameter of_Z: Z -> t.
+  Parameter to_Z: t -> Z.
+
 End VADDR.
